building x509

src/RIoT.X509.fst
@@ -3,7 +3,8 @@ module RIoT.X509
 open Common
 
 open LowStar.BufferOps
-open Lib.IntTypes
+open FStar.Integers
+//open Lib.IntTypes
 
 open Spec.Hash.Definitions
 open Hacl.Hash.Definitions
@@ -31,7 +32,7 @@ let _BIGLEN : I.uint_32 = 0x09ul
 
 noeq
 type bigval_t = {
-     data : B.lbuffer uint32 (v _BIGLEN)
+     data : B.lbuffer HI.uint32 (v _BIGLEN)
   }
 
 /// REF:
@@ -44,7 +45,7 @@ noeq
 type affine_point_t = {
      x: bigval_t;
      y: bigval_t;
-     infinity: B.pointer uint32
+     infinity: B.pointer HI.uint32
   }
 type riot_ecc_publickey = affine_point_t
 
@@ -78,30 +79,120 @@ let live_ecdsa_sig
   /\ B.live h s.s.data
 type live_ecc_privatekey = live_ecdsa_sig
 
+#set-options "--max_fuel 50 --max_ifuel 50"
+#push-options "--query_stats"
+(*)
+val memcpy: #a:eqtype -> src:B.buffer a -> dst:B.buffer a -> len:I.uint_32 -> HST.Stack unit
+  (requires fun h0 ->
+    let l_src = M.loc_buffer src in
+    let l_dst = M.loc_buffer dst in
+    B.live h0 src /\ B.live h0 dst /\
+    B.length src = I.v len /\
+    B.length dst = I.v len /\
+    M.loc_disjoint l_src l_dst)
+  (ensures fun h0 () h1 ->
+    let l_src = M.loc_buffer src in
+    let l_dst = M.loc_buffer dst in
+    B.live h1 src /\
+    B.live h1 dst /\
+    M.(modifies l_dst h0 h1) /\
+    S.equal (B.as_seq h1 dst) (B.as_seq h0 src))
+let memcpy #a src dst len =
+  let h0 = HST.get () in
+  let inv h (i: nat) =
+    B.live h src /\ B.live h dst /\
+    M.(M.modifies (M.loc_buffer dst) h0 h) /\
+    i <= I.v len /\
+    S.equal (Seq.slice (B.as_seq h src) 0 i) (Seq.slice (B.as_seq h dst) 0 i)
+  in
+  let body (i: I.uint_32{ 0 <= I.v i /\ I.v i < I.v len }): HST.Stack unit
+    (requires (fun h -> inv h (I.v i)))
+    (ensures (fun h0 () h1 -> inv h0 (I.v i) /\ inv h1 (I.v i + 1)))
+  =
+    let open B in
+    dst.(i) <- src.(i)
+  in
+  C.Loops.for 0ul len inv body
+*)
+let rec memcpy
+  (#a:eqtype)
+  (dst: B.buffer a)
+  (src: B.buffer a)
+  (len: I.uint_32)
+: HST.Stack unit
+  (requires fun h ->
+      B.live h dst
+    /\ B.live h src
+    /\ B.disjoint dst src
+    /\ len > 0ul
+    /\ len <= B.len src
+    /\ B.len src <= B.len dst)
+  (ensures  fun h0 _ h1 ->
+      M.modifies (M.loc_buffer dst) h0 h1
+/// TODO: /\ (S.slice (B.as_seq h1 dst) 0 (v len - 1)) `S.equal` (S.slice (B.as_seq h1 src) 0 (v len - 1))
+    )
+=
+  let cur = len - 1ul in
+  dst.(cur) <- src.(cur);
+  match cur with
+  | 0ul -> ()
+  | _   -> memcpy dst src cur
 
+#reset-options "--z3rlimit 50 --max_fuel 50 --max_ifuel 50"
 let riot_kdf_fixed
-  (fixed_size: I.uint_32{(v fixed_size) > 0})
-  (fixed: B.lbuffer uint8 (v fixed_size))
-  (label_size: I.uint_32)
-  (label: B.lbuffer uint8 (v label_size))
-  (context_size: I.uint_32)
-  (context: B.lbuffer uint8 (v context_size))
+  (#fixed_size: I.uint_32{(v fixed_size) > 0})
+  (fixed: B.lbuffer HI.uint8 (v fixed_size))
+  (#label_size: I.uint_32{(v label_size) > 0})
+  (label: B.lbuffer HI.uint8 (v label_size))
+  (#context_size: I.uint_32{(v context_size) > 0})
+  (context: B.lbuffer HI.uint8 (v context_size))
   (numberOfBits: I.uint_32)
+  (total_size: B.pointer I.uint_32)
 : HST.Stack unit
   (requires fun h ->
       B.live h fixed
     /\ B.live h label
     /\ B.live h context
+    /\ B.live h total_size
     /\ B.disjoint fixed label
     /\ B.disjoint fixed context
-    /\ B.disjoint context label)
+    /\ B.disjoint context label
+    /\ B.disjoint total_size fixed
+    /\ B.disjoint total_size label
+    /\ B.disjoint total_size context
+    /\ I.ok (+) label_size context_size
+    /\ I.ok (+) (label_size + context_size) 5ul
+/// REF: assert(fixedSize >= total);
+    /\ fixed_size >= (label_size + context_size + 5ul))
   (ensures  fun h0 _ h1 -> True)
 =
   HST.push_frame();
 
-  let total_size: I.uint_32 =
-      (if (!*fixed) = (u8 0x00) then fixed_size else 0ul)
-    + (if (!*label) = (u8 0x00) then label_size else 0ul) in
+/// REF: size_t  total = (((label) ? labelSize : 0) + ((context) ? contextSize : 0) + 5);
+  total_size.(0ul) <- label_size + context_size + 5ul;
+
+/// REF: if (label) {
+///        memcpy(fixed, label, labelSize);
+///        fixed += labelSize;
+///    }
+  //memcpy fixed label label_size;
+  let fixed' = B.sub fixed 0ul label_size in
+
+/// REF: *fixed++ = 0;
+  fixed'.(1ul) <- (HI.u8 0x00);
+
+/// REF: if (context) {
+///        memcpy(fixed, context, contextSize);
+///        fixed += contextSize;
+///      }
+  //memcpy fixed' context context_size;
+  let fixed'' = B.sub fixed 0ul label_size in
+
+/// REF: numberOfBits = UINT32_TO_BIGENDIAN(numberOfBits);
+
+/// REF: memcpy(fixed, &numberOfBits, 4);
+  //memcpy fixed''
+/// REF: return total;
 
   HST.pop_frame()
 
